experiments/lean/src/ddl/host/basic.lean
@@ -3,18 +3,23 @@ import ddl.basic
 namespace ddl.host
 
   /- The type syntax of the host language -/
-  inductive type : Type
-    | unit : type
-    | bool : type
-    | nat : type
-    | sum : type → type → type
-    | prod : type → type → type
-    | array : type → type
+  inductive type (ℓ : Type) : Type
+    | bool {} : type
+    | nat {} : type
+    | sum {} : type → type → type
+    | struct_nil {} : type
+    | struct_cons : ℓ → type → type → type
+    | array {} : type → type
 
   namespace type
 
-    instance : has_add type := ⟨type.sum⟩
-    instance : has_mul type := ⟨type.prod⟩
+    variables {ℓ : Type}
+
+    instance : has_add (type ℓ) := ⟨type.sum⟩
+
+    def lookup (l : ℓ) [decidable_eq ℓ] : type ℓ → option (type ℓ)
+      | (struct_cons l' t tr) := if l = l' then some t else lookup tr
+      | _                     := none
 
   end type
 
@@ -26,18 +31,21 @@ namespace ddl.host
 
 
   /- The expression syntax of the host language -/
-  inductive expr : Type
-    | bool : bool → expr
-    | nat : ℕ → expr
-    | app_binop : binop → expr → expr → expr
+  inductive expr (ℓ : Type) : Type
+    | bool {} : bool → expr
+    | nat {} : ℕ → expr
+    | app_binop {} : binop → expr → expr → expr
+    | proj : expr → ℓ → expr
 
-  instance has_coe_to_bool : has_coe bool expr := ⟨expr.bool⟩
-  instance has_coe_to_nat : has_coe ℕ expr  := ⟨expr.nat⟩
+  instance has_coe_to_bool {ℓ} : has_coe bool (expr ℓ) := ⟨expr.bool⟩
+  instance has_coe_to_nat {ℓ} : has_coe ℕ (expr ℓ)  := ⟨expr.nat⟩
 
   namespace expr
 
-    instance : has_add expr := ⟨app_binop binop.add⟩
-    instance : has_mul expr := ⟨app_binop binop.mul⟩
+    variables {ℓ : Type}
+
+    instance : has_add (expr ℓ) := ⟨app_binop binop.add⟩
+    instance : has_mul (expr ℓ) := ⟨app_binop binop.mul⟩
 
   end expr
 
