experiments/lean/src/ddl/host/typing.lean
@@ -2,25 +2,36 @@ import ddl.host.basic
 
 namespace ddl.host
 
-  inductive has_type : expr → type → Prop
-    | bool {b} :
-        has_type (expr.bool b) type.bool
-    | nat {n} :
-        has_type (expr.nat n) type.nat
-    | add {e₁ e₂} :
-        has_type e₁ type.nat →
-        has_type e₂ type.nat →
-        has_type (e₁ + e₂) type.nat
-    | mul {e₁ e₂} :
-        has_type e₁ type.nat →
-        has_type e₂ type.nat →
-        has_type (e₁ * e₂) type.nat
+  open ddl
 
+  section
+
+    variables {ℓ : Type} [decidable_eq ℓ]
+
+    inductive has_type : expr ℓ → type ℓ → Prop
+      | bool {b} :
+          has_type (expr.bool b) type.bool
+      | nat {n} :
+          has_type (expr.nat n) type.nat
+      | add {e₁ e₂} :
+          has_type e₁ type.nat →
+          has_type e₂ type.nat →
+          has_type (e₁ + e₂) type.nat
+      | mul {e₁ e₂} :
+          has_type e₁ type.nat →
+          has_type e₂ type.nat →
+          has_type (e₁ * e₂) type.nat
+      | proj {e₁ tr tf l} :
+          has_type e₁ tr →
+          type.lookup l tr = some tf →
+          has_type (expr.proj e₁ l) tf
+
+  end
 
   /- A correctly typed expression -/
-  structure typed_expr : Type :=
-    (e : expr)
-    (t : type)
+  structure typed_expr (ℓ : Type) [decidable_eq ℓ] : Type :=
+    (e : expr ℓ)
+    (t : type ℓ)
     (h : has_type e t)
 
 end ddl.host
