experiments/lean/src/ddl/binary/default.lean
@@ -1,6 +1,7 @@
 import ddl.binary.basic
 import ddl.binary.binder
 import ddl.binary.ctx
+import ddl.binary.formation
 import ddl.binary.kinding
 import ddl.binary.monad
 import ddl.binary.repr
