experiments/lean/src/ddl/binary/kinding.lean
@@ -4,50 +4,55 @@ import ddl.binary.binder
 import ddl.binary.ctx
 import ddl.binary.repr
 
-namespace ddl.binary.type
+namespace ddl.binary
 
   open ddl
   open ddl.binary
 
-  variables {α : Type}
+  section
 
-  inductive has_kind : ctx → type α → kind → Prop
-    | var {Γ} (x : ℕ) {k} :
-        ctx.lookup x Γ = some (binder.abs k) →
-        has_kind Γ x k
-    | unit {Γ} :
-        has_kind Γ type.unit ★
-    | bit {Γ} :
-        has_kind Γ type.bit ★
-    | sum {Γ t₁ t₂} :
-        has_kind Γ t₁ ★ →
-        has_kind Γ t₂ ★ →
-        has_kind Γ (t₁ + t₂) ★
-    | prod {Γ t₁ t₂} :
-        has_kind Γ t₁ ★ →
-        has_kind (Σ ⟦ t₂ ⟧ :: Γ) t₂ ★ →
-        has_kind Γ (Σ0: t₁, t₂) ★
-    | array {Γ t e} :
-        has_kind Γ t ★ →
-        host.has_type e host.type.nat →
-        has_kind Γ [ t; e ] ★
-    | cond {Γ t e} :
-        has_kind Γ t ★ →
-        host.has_type e host.type.bool →
-        has_kind Γ {0: t | e } ★
-    | abs {Γ t k₁ k₂} :
-        has_kind (Λ k₁ :: Γ) t k₁ →
-        has_kind Γ (Λ0: k₁, t) (k₁ ⇒ k₂)
-    | app {Γ t₁ t₂ k₁ k₂} :
-        has_kind Γ t₁ (k₁ ⇒ k₂) →
-        has_kind Γ t₂ k₁ →
-        has_kind Γ (t₁ ∙ t₂) k₂
+    variables {ℓ α : Type} [decidable_eq ℓ]
+
+    inductive has_kind : ctx ℓ → type ℓ α → kind → Prop
+      | bvar {Γ} (x : ℕ) {k} :
+          ctx.lookup x Γ = some (binder.abs k) →
+          has_kind Γ ↑x k
+      | bit {Γ} :
+          has_kind Γ type.bit ★
+      | sum {Γ t₁ t₂} :
+          has_kind Γ t₁ ★ →
+          has_kind Γ t₂ ★ →
+          has_kind Γ (t₁ + t₂) ★
+      | struct_nil {Γ} :
+          has_kind Γ type.struct_nil ★
+      | struct_cons {Γ l t₁ t₂} :
+          has_kind Γ t₁ ★ →
+          has_kind (Σ ⟦ t₂ ⟧ :: Γ) t₂ ★ →
+          has_kind Γ (type.struct_cons l t₁ t₂) ★
+      | array {Γ t e} :
+          has_kind Γ t ★ →
+          host.has_type e host.type.nat →
+          has_kind Γ [ t; e ] ★
+      | cond {Γ t e} :
+          has_kind Γ t ★ →
+          host.has_type e host.type.bool →
+          has_kind Γ {0: t | e } ★
+      | abs {Γ t k₁ k₂} :
+          has_kind (Λ k₁ :: Γ) t k₁ →
+          has_kind Γ (Λ0: k₁, t) (k₁ ⇒ k₂)
+      | app {Γ t₁ t₂ k₁ k₂} :
+          has_kind Γ t₁ (k₁ ⇒ k₂) →
+          has_kind Γ t₂ k₁ →
+          has_kind Γ (t₁ ∙ t₂) k₂
+
+  end
+
 
   /- A correctly kinded type -/
-  structure kinded (α : Type) : Type :=
-    (Γ : ctx)
-    (t : type α)
+  structure kinded_type (ℓ α : Type) [decidable_eq ℓ] : Type :=
+    (Γ : ctx ℓ)
+    (t : type ℓ α)
     (k : kind)
     (h : has_kind Γ t k)
 
-end ddl.binary.type
+end ddl.binary
