experiments/lean/src/ddl/binary/monad.lean
@@ -5,36 +5,38 @@ namespace ddl.binary.type
   open ddl
   open ddl.binary
 
-  variables {α β : Type}
+  variables {ℓ α β : Type}
 
-  def bind : type α → (α → type β) → type β
-    | (bvar i)      f := bvar i
-    | (fvar x)      f := (f x)
-    | (unit)        f := unit
-    | (bit)         f := bit
-    | (sum t₁ t₂)   f := sum (bind t₁ f) (bind t₂ f)
-    | (prod t₁ t₂)  f := prod (bind t₁ f) (bind t₂ f)
-    | (array t e)   f := array (bind t f) e
-    | (cond t e)    f := cond (bind t f) e
-    | (abs k t)     f := abs k (bind t f)
-    | (app t₁ t₂)   f := app (bind t₁ f) (bind t₂ f)
 
-  instance : monad type :=
-    { pure := @fvar
-    , bind := @bind
+  def bind : type ℓ α → (α → type ℓ β) → type ℓ β
+    | (bvar i)              f := bvar i
+    | (fvar x)              f := (f x)
+    | (bit)                 f := bit
+    | (sum t₁ t₂)           f := sum (bind t₁ f) (bind t₂ f)
+    | (struct_nil)          f := struct_nil
+    | (struct_cons l t₁ t₂) f := struct_cons l (bind t₁ f) (bind t₂ f)
+    | (array t e)           f := array (bind t f) e
+    | (cond t e)            f := cond (bind t f) e
+    | (abs k t)             f := abs k (bind t f)
+    | (app t₁ t₂)           f := app (bind t₁ f) (bind t₂ f)
+
+
+  instance : monad (type ℓ) :=
+    { pure := @fvar ℓ
+    , bind := @bind ℓ
     , id_map := begin
         intros α t,
         simp [bind, function.comp],
         induction t,
           case bvar i { exact rfl },
           case fvar x { exact rfl },
-          case unit { exact rfl },
           case bit { exact rfl },
           case sum t₁ t₂ ht₁ ht₂ {
             simp [bind, function.comp],
             rw [ht₁, ht₂],
           },
-          case prod t₁ t₂ ht₁ ht₂ {
+          case struct_nil { exact rfl },
+          case struct_cons l t₁ t₂ ht₁ ht₂ {
             simp [bind, function.comp],
             rw [ht₁, ht₂],
           },
@@ -61,14 +63,14 @@ namespace ddl.binary.type
         induction t,
           case bvar i { exact rfl },
           case fvar x { exact rfl },
-          case unit { exact rfl },
           case bit { exact rfl },
           case sum t₁ t₂ ht₁ ht₂ {
             simp [bind],
             simp [bind] at ht₁ ht₂,
             rw [ht₁, ht₂]
           },
-          case prod t₁ t₂ ht₁ ht₂ {
+          case struct_nil { exact rfl },
+          case struct_cons l t₁ t₂ ht₁ ht₂ {
             simp [bind],
             simp [bind] at ht₁ ht₂,
             rw [ht₁, ht₂]
