experiments/lean/src/ddl/binary/subst.lean
@@ -3,78 +3,83 @@ import ddl.binary.monad
 
 namespace ddl.binary
 
-  open ddl.binary
+  -- open ddl.binary
 
   namespace type
 
-    variables {α : Type} [decidable_eq α]
+    variables {ℓ α : Type} [decidable_eq α]
 
-    def open_var : ℕ → α → type α → type α
+
+    def open_var : ℕ → α → type ℓ α → type ℓ α
       | i x (bvar i') := if i = i' then fvar x else bvar i'
       | i x (fvar x') := fvar x'
-      | i x (unit) := unit
       | i x (bit) := bit
       | i x (sum t₁ t₂) := sum (open_var i x t₁) (open_var i x t₂)
-      | i x (prod t₁ t₂) := prod (open_var i x t₁) (open_var i x t₂)
+      | i x (struct_nil) := struct_nil
+      | i x (struct_cons l t₁ t₂) := struct_cons l (open_var i x t₁) (open_var i x t₂)
       | i x (array t e) := array (open_var i x t) e
       | i x (cond t e) := cond (open_var i x t) e
       | i x (abs k t) := abs k (open_var (i + 1) x t)
       | i x (app t₁ t₂) := app (open_var i x t₁) (open_var i x t₂)
 
-    def close_var : ℕ → α → type α → type α
+
+    def close_var : ℕ → α → type ℓ α → type ℓ α
       | i x (bvar i') := bvar i'
       | i x (fvar x') := if x = x' then bvar i else fvar x'
-      | i x (unit) := unit
       | i x (bit) := bit
       | i x (sum t₁ t₂) := sum (close_var i x t₁) (close_var i x t₂)
-      | i x (prod t₁ t₂) := prod (close_var i x t₁) (close_var i x t₂)
+      | i x (struct_nil) := struct_nil
+      | i x (struct_cons l t₁ t₂) := struct_cons l (close_var i x t₁) (close_var i x t₂)
       | i x (array t e) := array (close_var i x t) e
       | i x (cond t e) := cond (close_var i x t) e
       | i x (abs k t) := abs k (close_var (i + 1) x t)
       | i x (app t₁ t₂) := app (close_var i x t₁) (close_var i x t₂)
 
+
     theorem close_open_var :
-      Π (x : α) (t : type α),
+      Π (x : α) (t : type ℓ α),
       close_var 0 x (open_var 0 x t) = t :=
     begin
       intros x t,
       induction t,
-        case bvar i { exact sorry },
-        case fvar x { exact sorry },
-        case unit { exact sorry },
-        case bit { exact sorry },
-        case sum t₁ t₂ ht₁ ht₂ { exact sorry },
-        case prod t₁ t₂ ht₁ ht₂ { exact sorry },
-        case array t e ht { exact sorry },
-        case cond t e ht { exact sorry },
-        case abs k t ht { exact sorry },
-        case app t₁ t₂ ht₁ ht₂ { exact sorry },
+        case bvar i { admit },
+        case fvar x { admit },
+        case bit { admit },
+        case sum t₁ t₂ ht₁ ht₂ { admit },
+        case struct_nil { admit },
+        case struct_cons l t₁ t₂ ht₁ ht₂ { admit },
+        case array t e ht { admit },
+        case cond t e ht { admit },
+        case abs k t ht { admit },
+        case app t₁ t₂ ht₁ ht₂ { admit },
     end
 
+
     theorem open_close_var :
-      Π (x : α) (t : type α),
+      Π (x : α) (t : type ℓ α),
       open_var 0 x (close_var 0 x t) = t :=
     begin
       intros x t,
       induction t,
-        case bvar i { exact sorry },
-        case fvar x {  exact sorry },
-        case unit { exact sorry },
-        case bit { exact sorry },
-        case sum t₁ t₂ ht₁ ht₂ { exact sorry },
-        case prod t₁ t₂ ht₁ ht₂ { exact sorry },
-        case array t e ht { exact sorry },
-        case cond t e ht { exact sorry },
-        case abs k t ht { exact sorry },
-        case app t₁ t₂ ht₁ ht₂ { exact sorry },
+        case bvar i { admit },
+        case fvar x {  admit },
+        case bit { admit },
+        case sum t₁ t₂ ht₁ ht₂ { admit },
+        case struct_nil { admit },
+        case struct_cons l t₁ t₂ ht₁ ht₂ { admit },
+        case array t e ht { admit },
+        case cond t e ht { admit },
+        case abs k t ht { admit },
+        case app t₁ t₂ ht₁ ht₂ { admit },
     end
 
-    def subst (x : α) (src : type α) (dst : type α) : type α :=
+
+    def subst (x : α) (src : type ℓ α) (dst : type ℓ α) : type ℓ α :=
       dst >>= λ x', if x' = x then src else (fvar x)
 
     notation `[ ` x ` ↦ ` src ` ]` dst := subst x src dst
 
-    example {x: α} {t : type α} :
+    example {x: α} {t : type ℓ α} :
         ([x ↦ t] Λ0: ★, ↑0 ∙ ↑x) = (Λ0: ★, ↑0 ∙ t) := sorry
 
   end type
