experiments/lean/src/ddl/host/formation.lean
@@ -1,0 +1,51 @@
+import ddl.host.typing
+
+namespace ddl.host
+
+  open ddl
+  open ddl.host
+
+  namespace type
+
+    variables {ℓ : Type} [decidable_eq ℓ]
+
+
+    inductive struct : type ℓ → Prop
+      | nil {} : struct struct_nil
+      | cons {l t₁ t₂} : struct (struct_cons l t₁ t₂)
+
+
+    inductive well_formed : type ℓ → Prop
+      | bool {} :
+          well_formed bool
+      | nat {} :
+          well_formed nat
+      | sum {t₁ t₂} :
+          well_formed t₁ →
+          well_formed t₂ →
+          well_formed (sum t₁ t₂)
+      | struct_nil {} :
+          well_formed struct_nil
+      | struct_cons {l t₁ t₂} :
+          well_formed t₁ →
+          well_formed t₂ →
+          struct t₂ →
+          well_formed (struct_cons l t₁ t₂)
+      | array {t} :
+          well_formed t →
+          well_formed (array t)
+
+
+    lemma well_formed_lookup :
+        Π {l : ℓ} {tr tf : type ℓ},
+        well_formed tr →
+        lookup l tr = some tf →
+        well_formed tf :=
+      begin
+        admit
+      end
+
+
+  end type
+
+end ddl.host
