experiments/lean/src/ddl/host/lemmas.lean
@@ -1,58 +1,95 @@
-import ddl.host.typing
+import ddl.host.formation
 import ddl.host.evaluation
+import ddl.host.typing
 
 namespace ddl.host
+
+  open ddl
+
+  variables {ℓ α : Type} [decidable_eq ℓ]
+
+
+  -- WELL-FORMEDNESS
+  -- https://softwarefoundations.cis.upenn.edu/plf-current/Records.html#lab348
+
+  lemma has_type_well_formed :
+      Π (e : expr ℓ) (t : type ℓ),
+      has_type e t →
+      type.well_formed t :=
+    begin
+      admit
+    end
+
+
+  -- WELL-FORMEDNESS
+  -- https://softwarefoundations.cis.upenn.edu/plf-current/Records.html#lab348
+
+  lemma lookup_field_in_value :
+      Π (v : expr ℓ) (l : ℓ) (tr tf : type ℓ),
+      value v →
+      has_type v tr →
+      type.lookup l tr = some tf →
+      ∃ ef, /- expr.lookup l v = some ef ∧ -/ has_type ef tf :=
+    begin
+      admit
+    end
 
   -- PROGRESS
   -- https://softwarefoundations.cis.upenn.edu/plf-current/StlcProp.html#lab220
 
   theorem progress :
-    Π (e : expr) (t : type),
-    has_type e t →
-    value e ∨ ∃ e', e ⟹ e' :=
-  begin
-    intros e t ht,
-    induction ht,
-      case has_type.bool bv {
-        apply or.inl,
-        exact value.bool bv
-      },
-      case has_type.nat nv {
-        apply or.inl,
-        exact value.nat nv
-      },
-      case has_type.add e₁ e₂ ht₁ ht₂ hp₁ hp₂ {
-        exact sorry
-      },
-      case has_type.mul e₁ e₂ ht₁ ht₂ hp₁ hp₂ {
-        exact sorry
-      },
-  end
+      Π (e : expr ℓ) (t : type ℓ),
+      has_type e t →
+      value e ∨ ∃ e', e ⟹ e' :=
+    begin
+      intros e t ht,
+      induction ht,
+        case has_type.bool bv {
+          apply or.inl,
+          exact value.bool bv
+        },
+        case has_type.nat nv {
+          apply or.inl,
+          exact value.nat nv
+        },
+        case has_type.add e₁ e₂ ht₁ ht₂ hp₁ hp₂ {
+          admit
+        },
+        case has_type.mul e₁ e₂ ht₁ ht₂ hp₁ hp₂ {
+          admit
+        },
+        case has_type.proj e₁ tr tf l ht₁ hl hp₁ {
+          admit
+        }
+    end
 
 
   -- PRESERVATION
   -- https://softwarefoundations.cis.upenn.edu/plf-current/StlcProp.html#lab222
 
   theorem preservation :
-    Π (e e' : expr) (t : type),
-    has_type e t →
-    e ⟹ e' →
-    has_type e' t :=
-  begin
-    intros e e' t ht hs,
-    induction ht,
-      case has_type.bool bv hsbv {
-        exact sorry,
-      },
-      case has_type.nat hsnat {
-        exact sorry
-      },
-      case has_type.add e₁ e₂ ht₁ ht₂ hs₁ hs₂ {
-        exact sorry
-      },
-      case has_type.mul e₁ e₂ ht₁ ht₂ hs₁ hs₂ {
-        exact sorry
-      },
-  end
+      Π (e e' : expr ℓ) (t : type ℓ),
+      has_type e t →
+      e ⟹ e' →
+      has_type e' t :=
+    begin
+      intros e e' t ht hs,
+      induction ht,
+        case has_type.bool bv hsbv {
+          admit,
+        },
+        case has_type.nat hsnat {
+          admit,
+        },
+        case has_type.add e₁ e₂ ht₁ ht₂ hs₁ hs₂ {
+          admit,
+        },
+        case has_type.mul e₁ e₂ ht₁ ht₂ hs₁ hs₂ {
+          admit,
+        },
+        case has_type.proj e₁ tr tf l ht₁ hl hs₁ {
+          admit,
+        }
+    end
 
 end ddl.host
