experiments/lean/src/ddl/parsing.lean
@@ -3,7 +3,7 @@ import ddl.binary
 namespace ddl
 
   -- FIXME: constrain `kt.embed` to be `Type 0`
-  def parse {α : Type} : Π (kt : binary.type.kinded α), list bool → /- kt.embed -/ sorry :=
+  def parse {ℓ α} [decidable_eq ℓ] : Π (kt : binary.kinded_type ℓ α), list bool → /- kt.embed -/ sorry :=
     sorry
 
 end ddl
